DerivationHelpers.v
@@ -373,6 +373,47 @@ Proof.
 Qed.
 Hint Resolve support_open2: sets.
 
+
+Lemma subset_nil : forall {T} A, @subset T nil A.
+Proof.
+  steps. eauto with sets.
+Qed.
+
+Lemma in_subset_not:
+  forall {T} (l1 l2: list T) (x: T),
+    subset l1 l2 -> not (x ∈ l2) -> not (x ∈ l1).
+Proof.
+  steps.
+Qed.
+Hint Resolve in_subset_not: sets.
+Hint Unfold fv: deriv.
+
+Lemma subset_open_open: forall k1 k2 t n3 n2 n1 A,
+    subset (fv (open k1 (open k2 t (fvar n3 term_var)) (fvar n2 term_var))) (n1::n2::n3::A) ->
+    ~ n3 ∈ (fv t) ->
+    ~ n2 ∈ (fv t) ->
+    ~ n1 ∈ (fv t) ->
+    subset (fv t) A.
+  intros.
+  apply (subset_add5 _ n1 n2 n3 _ _ H2 H1 H0).
+  pose proof (proj2
+                (iff_and (singleton_subset (n1::n2::n3::A) n2))
+                (inList2 n2 n1 (n3::A))) as H_temp1.
+  pose proof (proj2
+                (iff_and (singleton_subset (n1::n2::n3::A) n3))
+                (inList3 n3 n2 n1 (A))) as H_temp2.
+  rewrite <- (pfv_fvar n2 term_var) in H_temp1.
+  rewrite <- (pfv_fvar n3 term_var) in H_temp2.
+  pose proof (support_open (open k2 t (fvar n3 term_var)) (fvar n2 term_var) term_var k1 _ H H_temp1) as H_temp3.
+  apply (support_open t (fvar n3 term_var) term_var k2 (n1::n2::n3::A) H_temp3 H_temp2).
+Qed.
+
+Hint Rewrite fv_context_append: deriv.
+
+
+
+
+
 Require Import Coq.Lists.List.
 
 Fixpoint NoDupb l : bool :=
@@ -439,7 +480,8 @@ Proof.
 Qed.
 
 Ltac inst_list_prop:=
- match goal with
+  match goal with
+  | H: forall x, x ∈ nil -> _ |- _ => clear H
   | H: forall x, x ∈ ?a1::nil ->  _ |- _ =>
     pose proof (H a1 (inList1 a1 nil)); clear H
   | H: forall x, x ∈ ?a1::?a2::nil -> _ |- _ =>
